CoqOfRust/core/slice/links/mod.v
@@ -1,6 +1,8 @@
 Require Import CoqOfRust.CoqOfRust.
 Require Import links.M.
 Require Import core.slice.mod.
+Require Import core.slice.links.index.
+Require core.links.option.
 Import Run.
 
 Module Impl_Slice.
@@ -14,4 +16,18 @@ Module Impl_Slice.
         index.get(self)
     }
   *)
+  Definition run_get 
+      {T : Set} `{Link T}
+      {I : Set} `{Link I} 
+      {Output : Set} `{Link Output}
+      (run_SliceIndex_for_Self : SliceIndex.Run I (T := Self T) (Output := Output))
+      (self : Ref.t Pointer.Kind.Ref (Self T)) 
+      (index : I) :
+    {{ slice.Impl_slice_T.get (Φ T) [] [ Φ I ] [ φ self; φ index ] 🔽 option Output }}.
+  Proof.
+    destruct run_SliceIndex_for_Self.
+    destruct get as [get [H_get run_get]].
+    run_symbolic.
+    eapply Run.CallPrimitiveGetTraitMethod.
+
 End Impl_Slice.
